mutable_typed_shared_data: Add assertion on load

theories/examples/mutable_typed_shared_data/load.v
@@ -1,5 +1,6 @@
 From iris.proofmode Require Import proofmode.
 From cap_machine Require Import fundamental logrel macros macros_helpers proofmode rules register_tactics.
+From cap_machine.examples Require Import template_adequacy template_adequacy_ocpl.
 From cap_machine.examples.mutable_typed_shared_data Require Import dynamic_checks invariants.
 
 Section load_cap.
@@ -16,30 +17,45 @@ Section load_cap.
 
   (* Instructions to load in `r_t1` the capability store in the seal `r_t1`, sealed by the hidden `WSealRange` placed at `off_seal`. *)
   (* This will return a new sealed value in `r_t1` and override the registers r_t2`. *)
-  Definition load_global_macro_cap_closure_instrs (off_seal : Z) :=
+  Definition load_global_macro_cap_closure_instrs (fptr_assert : Z) (off_seal : Z) :=
     encodeInstrsW [
       Mov r_t2 r_t1;
       Mov r_t1 PC;
       Lea r_t1 (off_seal - 1)%Z;
       Load r_t1 r_t1
     ] ++ load_global_macro_cap_instrs ++ encodeInstrsW [
-      Mov r_t1 r_t2;
-      Mov r_t2 0;
+      (* Prepare the registers for the `assert` macro. *)
+      IsPtr r_t4 r_t2;
+      Mov r_t5 1;
+      (* Save registers *)
+      Mov r_t6 r_t2
+    ] ++ assert_instrs fptr_assert ++ encodeInstrsW [
+      Mov r_t1 r_t6;
+      Mov r_t6 0;
       Jmp r_t0
     ].
 
+  (* Assert invariant *)
+  Definition assert_inv b_a e_a a_flag :=
+    na_inv logrel_nais ocpl.assertN (assert_inv b_a a_flag e_a).
+
+  Definition flag_inv a_flag flagN := inv flagN (a_flag ↦ₐ WInt 0%Z).
+
+
   Lemma load_global_macro_cap_spec
     p_pc b_pc e_pc a_pc       (* PC *)
-    a_cap                     (* Address *)
+    a_cap                     (* Addresses *)
     p_seal b_seal e_seal τ Φ  (* Seal capability *)
     φ:
 
     let instrs := load_global_macro_cap_instrs in
     let scap := SCap RW a_cap (a_cap ^+ 1)%a a_cap in
 
+    (* Validity PC *)
     ExecPCPerm p_pc →
     SubBounds b_pc e_pc a_pc (a_pc ^+ (length instrs))%a →
 
+    (* Validity `WSealRange` *)
     permit_unseal p_seal = true →
     withinBounds b_seal e_seal τ = true →
     withinBounds a_cap (a_cap ^+ 1)%a a_cap = true →
@@ -50,6 +66,7 @@ Section load_cap.
       ∗ r_t1 ↦ᵣ WSealRange p_seal b_seal e_seal τ
       ∗ r_t2 ↦ᵣ WSealed τ scap
 
+      (* Seal invariant *)
       ∗ ▷ (valid_sealed (WSealed τ scap) τ Φ)
       ∗ seal_pred_cap τ
       ∗ na_own logrel_nais ⊤
@@ -100,23 +117,32 @@ Section load_cap.
   Qed.
 
   Lemma load_global_macro_cap_closure_spec (off_seal : Z)
-    p_pc b_pc e_pc a_pc  (* PC *)
-    a_seal a_cap         (* Addresses *)
-    p_seal τ Φ           (* Seal capability *)
-    adv w2               (* Values in registers *)
+    p_pc b_pc e_pc a_pc               (* PC *)
+    a_seal a_cap                      (* Addresses *)
+    p_seal τ Φ                        (* Seal capability *)
+    adv w2 w3 w4 w5 w6                (* Values in registers *)
+    f_a b_a e_a a_flag flagN          (* Assert *)
+    b_link a_link e_link assert_entry (* Linking *)
     φ:
 
-    let instrs := load_global_macro_cap_closure_instrs off_seal in
+    let instrs := load_global_macro_cap_closure_instrs f_a off_seal in
     let scap := SCap RW a_cap (a_cap ^+ 1)%a a_cap in
 
+    (* Validity PC *)
     ExecPCPerm p_pc →
     ContiguousRegion a_pc (length instrs) →
     SubBounds b_pc e_pc a_pc (a_pc ^+ (length instrs))%a →
 
+    (* Validity linking table *)
+    (a_link + f_a)%a = Some assert_entry →
+    withinBounds b_link e_link assert_entry = true →
+
+    (* Validity `WSealRange` *)
     permit_unseal p_seal = true →
     withinBounds a_cap (a_cap ^+ 1)%a a_cap = true →
     withinBounds τ (τ ^+ 1)%ot τ = true →
 
+    (* Validity `WSealRange` location *)
     (a_pc + off_seal)%a = Some a_seal →
     withinBounds b_pc e_pc a_seal = true →
 
@@ -127,7 +153,20 @@ Section load_cap.
       ∗ r_t0 ↦ᵣ adv
       ∗ r_t1 ↦ᵣ WSealed τ scap
       ∗ r_t2 ↦ᵣ w2
+      ∗ r_t3 ↦ᵣ w3
+      ∗ r_t4 ↦ᵣ w4
+      ∗ r_t5 ↦ᵣ w5
+      ∗ r_t6 ↦ᵣ w6
 
+      (* Assert invariant *)
+      ∗ assert_inv b_a e_a a_flag
+      ∗ flag_inv a_flag flagN
+
+      (* Linking table *)
+      ∗ b_pc ↦ₐ WCap RO b_link e_link a_link
+      ∗ assert_entry ↦ₐ WCap E b_a e_a b_a
+
+      (* Seal invariant *)
       ∗ ▷ (valid_sealed (WSealed τ scap) τ Φ)
       ∗ seal_pred_cap τ
       ∗ na_own logrel_nais ⊤
@@ -138,6 +177,10 @@ Section load_cap.
              ∗ r_t0 ↦ᵣ adv
              ∗ (∃ w, r_t1 ↦ᵣ w ∗ ⌜is_cap w⌝ ∗ interp w)
              ∗ r_t2 ↦ᵣ WInt 0
+             ∗ r_t3 ↦ᵣ WInt 0
+             ∗ r_t4 ↦ᵣ WInt 0
+             ∗ r_t5 ↦ᵣ WInt 0
+             ∗ r_t6 ↦ᵣ WInt 0
 
              ∗ sealed_cap (WSealable scap)
              ∗ na_own logrel_nais ⊤
@@ -145,8 +188,9 @@ Section load_cap.
              -∗ WP Seq (Instr Executable) {{ λ v, φ v }})
     -∗ WP Seq (Instr Executable) {{ λ v, φ v }}.
   Proof.
-    iIntros (? ? ? Hbounds ? ? ? ? ? ?)
-      "(HPC & Hprog & Hseal & Hr_t0 & Hr_t1 & Hr_t2 & Hseal_valid & Hseal_pred & Hna & Hφ)".
+    iIntros (? ? ? Hbounds ? ? ? ? ? ? ? ?)
+      "(HPC & Hprog & Hseal & Hr_t0 & Hr_t1 & Hr_t2 & Hr_t3 & Hr_t4 & Hr_t5 & Hr_t6 &
+        Hassert_inv & Hflag_inv & Hlink & Hassert_link & Hseal_valid & Hseal_pred & Hna & Hφ)".
 
     iAssert (codefrag a_pc instrs) with "[Hprog]" as "Hprog"; [ iFrame |].
 
@@ -154,7 +198,7 @@ Section load_cap.
     focus_block_0 "Hprog" as "Hblock" "Hcont".
 
     iGo "Hblock".
-    { transitivity (a_pc + off_seal)%a; [ solve_addr +H6 | eauto ]. }
+    { transitivity (a_pc + off_seal)%a; [ solve_addr +H8 | eauto ]. }
 
     iInstr "Hblock".
 
@@ -165,13 +209,35 @@ Section load_cap.
     iApply load_global_macro_cap_spec; last iFrame "Hseal_valid ∗"; eauto.
 
     iIntros "!> (HPC & Hblock & Hr_t1 & Hr_t2 & Hseal_cap & Hna)".
-    iDestruct "Hr_t2" as (v) "(Hr_t2 & ?)".
+    iDestruct "Hr_t2" as (v) "(Hr_t2 & % & Hinterp)".
 
     unfocus_block "Hblock" "Hcont" as "Hprog".
 
     focus_block 2%nat "Hprog" as addr_block2 Haddr_block2 "Hblock" "Hcont".
 
-    iInstr "Hblock".
+    iGo "Hblock".
+
+    unfocus_block "Hblock" "Hcont" as "Hprog".
+
+    focus_block 3%nat "Hprog" as addr_block3 Haddr_block3 "Hblock" "Hcont".
+
+    iCombine "Hlink" "Hassert_link" as "Hlink".
+    iMod (na_inv_alloc logrel_nais _ seal_capN with "Hlink") as "#Hlink_inv".
+
+    iMod (na_inv_acc with "Hlink_inv Hna") as "(>(Hlink & Hassert_entry) & Hna & Hclose)"; [ solve_ndisj.. |].
+
+    iApply assert_success; last iFrame; [ eauto .. | solve_ndisj | by destruct is_cap |].
+    2: { apply contiguous_between_region_addrs; solve_addr +. }
+    1: { split; eauto. solve_addr +H11 H13. }
+
+    iIntros "!> (Hr_t0 & Hr_t1 & Hr_t2 & Hr_t3 & Hr_t4 & Hr_t5 & HPC & Hblock & Hna & Hlink & Hassert_entry)".
+
+    iMod ("Hclose" with "[$Hna $Hlink $Hassert_entry]") as "Hna".
+
+    iAssert (codefrag addr_block3 (assert_instrs f_a)) with "[$Hblock]" as "Hblock".
+    unfocus_block "Hblock" "Hcont" as "Hprog".
+
+    focus_block 4%nat "Hprog" as addr_block4 Haddr_block4 "Hblock" "Hcont".
 
     iGo "Hblock".
 
@@ -182,27 +248,36 @@ Section load_cap.
   Qed.
 
   Lemma load_global_macro_cap_closure_spec_full (off_seal : Z)
-    p_pc b_pc e_pc a_pc  (* PC *)
-    a_seal a_cap         (* Addresses *)
-    p_seal τ             (* Seal capability *)
-    adv w2               (* Values in registers *)
+    p_pc b_pc e_pc a_pc               (* PC *)
+    a_seal a_cap                      (* Addresses *)
+    p_seal τ                          (* Seal capability *)
+    adv                               (* Values in registers *)
+    f_a b_a e_a a_flag flagN          (* Assert *)
+    b_link a_link e_link assert_entry (* Linking *)
     rmap:
 
-    let instrs := load_global_macro_cap_closure_instrs off_seal in
+    let instrs := load_global_macro_cap_closure_instrs f_a off_seal in
     let scap := SCap RW a_cap (a_cap ^+ 1)%a a_cap in
 
+    (* Validity PC *)
     ExecPCPerm p_pc →
     ContiguousRegion a_pc (length instrs) →
     SubBounds b_pc e_pc a_pc (a_pc ^+ (length instrs))%a →
 
+    (* Validity linking table *)
+    (a_link + f_a)%a = Some assert_entry →
+    withinBounds b_link e_link assert_entry = true →
+
+    (* Validity `WSealRange` *)
     permit_unseal p_seal = true →
     withinBounds a_cap (a_cap ^+ 1)%a a_cap = true →
     withinBounds τ (τ ^+ 1)%ot τ = true →
 
+    (* Validity `WSealRange` location *)
     (a_pc + off_seal)%a = Some a_seal →
     withinBounds b_pc e_pc a_seal = true →
 
-    dom rmap = all_registers_s ∖ {[ PC; r_t0; r_t1; r_t2 ]} →
+    dom rmap = all_registers_s ∖ {[ PC; r_t0; r_t1 ]} →
 
     ⊢ (PC ↦ᵣ WCap p_pc b_pc e_pc a_pc
       ∗ region_mapsto a_pc (a_pc ^+ length instrs)%a instrs
@@ -210,8 +285,16 @@ Section load_cap.
       ∗ a_seal ↦ₐ WSealRange p_seal τ (τ ^+ 1)%ot τ
       ∗ r_t0 ↦ᵣ adv ∗ interp adv
       ∗ r_t1 ↦ᵣ WSealed τ scap ∗ interp (WSealed τ scap)
-      ∗ r_t2 ↦ᵣ w2
 
+      (* Assert invariant *)
+      ∗ assert_inv b_a e_a a_flag
+      ∗ flag_inv a_flag flagN
+
+      (* Linking table *)
+      ∗ b_pc ↦ₐ WCap RO b_link e_link a_link
+      ∗ assert_entry ↦ₐ WCap E b_a e_a b_a
+
+      (* Seal invariant *)
       ∗ seal_pred_cap τ
       ∗ na_own logrel_nais ⊤
 
@@ -220,10 +303,14 @@ Section load_cap.
       -∗ WP Seq (Instr Executable)
             {{ v, ⌜v = HaltedV⌝ → ∃ r: Reg, full_map r ∧ registers_mapsto r ∗ na_own logrel_nais ⊤ }})%I.
   Proof.
-    iIntros (? ? ? Hbounds ? ? ? ? ? ? Hdom)
-      "(HPC & Hprog & Hseal & Hr_t0 & #Hadv_interp & Hr_t1 & #Hseal_interp & Hr_t2 & Hseal_pred & Hna & Hrmap)".
+    iIntros (? ? ? Hbounds ? ? ? ? ? ? ? ? Hdom)
+      "(HPC & Hprog & Hseal & Hr_t0 & #Hadv_interp & Hr_t1 & #Hseal_interp &
+        Hassert_inv & Hflag_inv & Hlink & Hassert_link & Hseal_pred & Hna & Hrmap)".
 
     iDestruct (jmp_to_unknown with "Hadv_interp") as "Cont".
+
+    iExtractList "Hrmap" [r_t2; r_t3; r_t4; r_t5; r_t6]
+      as ["[Hr_t2 _]"; "[Hr_t3 _]"; "[Hr_t4 _]"; "[Hr_t5 _]"; "[Hr_t6 _]"].
 
     iAssert (∃ Φ, ▷ valid_sealed (WSealed τ scap) τ Φ)%I as (Φ) "-#Hseal_valid".
     { iDestruct (interp_valid_sealed with "Hseal_interp") as (Φ) "Hseal_valid".
@@ -231,17 +318,21 @@ Section load_cap.
 
     iApply load_global_macro_cap_closure_spec; last iFrame; eauto.
 
-    iIntros "!> (HPC & Hprog & Hr_t0 & Hr_t1 & Hr_t2 & Hseal_cap & Hna)".
+    iIntros "!> (HPC & Hprog & Hr_t0 & Hr_t1 & Hr_t2 & Hr_t3 & Hr_t4 & Hr_t5 & Hr_t6 & Hseal_cap & Hna)".
     iDestruct "Hr_t1" as (v) "(Hr_t1 & _ & Hinterp)".
 
     iApply "Cont"; [| iFrame "HPC Hna" ]; revgoals.
     { iAssert (interp (WInt 0)) as "Hinterp_int".
       { by rewrite !fixpoint_interp1_eq. }
 
+      iCombine "Hr_t6 Hinterp_int" as "Hr_t6".
+      iCombine "Hr_t5 Hinterp_int" as "Hr_t5".
+      iCombine "Hr_t4 Hinterp_int" as "Hr_t4".
+      iCombine "Hr_t3 Hinterp_int" as "Hr_t3".
       iCombine "Hr_t2 Hinterp_int" as "Hr_t2".
       iCombine "Hr_t1 Hinterp" as "Hr_t1".
       iCombine "Hr_t0 Hadv_interp" as "Hr_t0".
-      iInsertList "Hrmap" [r_t0; r_t1; r_t2].
+      iInsertList "Hrmap" [r_t0; r_t1; r_t2; r_t3; r_t4; r_t5; r_t6].
 
       iFrame. }
 
